src/asn1/ASN1.Low.Length.fst
@@ -1,0 +1,77 @@
+module ASN1.Low.Length
+///
+/// ASN.1 Low
+///
+open LowParse.Low.Base
+open LowParse.Low.Combinators
+module LDER = LowParse.Low.DER
+module SDER = LowParse.Spec.DER
+
+open ASN1.Base
+open ASN1.Spec.Length
+open ASN1.Low.Base
+
+module HS = FStar.HyperStack
+module HST = FStar.HyperStack.ST
+module B = LowStar.Buffer
+open FStar.Integers
+
+#reset-options "--max_fuel 0 --max_ifuel 0"
+
+#push-options "--z3rlimit 16"
+let offset_of_asn1_length
+  (len: asn1_int32)
+: Pure (offset: size_t{v offset == Seq.length (serialize serialize_asn1_length len)})
+  (requires True)
+  (ensures fun offset -> v offset == Seq.length (serialize serialize_asn1_length len))
+= serialize_asn1_length_unfold len;
+  let x = SDER.tag_of_der_length32_impl len in
+  if x < 128uy then
+  ( 1ul )
+  else if x = 129uy then
+  ( 2ul )
+  else if x = 130uy then
+  ( 3ul )
+  else if x = 131uy then
+  ( 4ul )
+  else
+  ( 5ul )
+#pop-options
+
+let serialize32_asn1_length ()
+: Tot (serializer32 serialize_asn1_length)
+= LDER.serialize32_bounded_der_length32 asn1_length_min asn1_length_max
+
+#push-options "--z3rlimit 32"
+let serialize32_asn1_length_backwards ()
+: Tot (serializer32_backwards serialize_asn1_length)
+= fun (len: asn1_int32)
+    (#rrel #rel: _)
+    (b: B.mbuffer byte_t rrel rel)
+    (pos: size_t)
+-> let offset = offset_of_asn1_length len in
+   (* Prf *) let h0 = HST.get () in
+   let offset = serialize32_asn1_length () len b (pos - offset) in
+   (* Prf *) let h1 = HST.get () in
+   (* Prf *) B.modifies_buffer_from_to_elim
+             (* buf *) b
+             (*frame*) 0ul (pos - offset)
+             (* new *) (B.loc_buffer_from_to
+                        (* buf *) b
+                        (*range*) (pos - offset) (pos))
+             (* mem *) h0 h1;
+   (* Prf *) B.modifies_buffer_from_to_elim
+             (* buf *) b
+             (*frame*) pos (u (B.length b))
+             (* new *) (B.loc_buffer_from_to
+                        (* buf *) b
+                        (*range*) (pos - offset) (pos))
+             (* mem *) h0 h1;
+   (* Prf *) writable_modifies
+             (* buf *) b
+             (* new *) (v (pos - offset)) (v (pos))
+             (* mem *) h0
+             (* loc *) B.loc_none
+             (* mem'*) h1;
+(* return *) offset
+#pop-options
