src/asn1/ASN1.Low.NULL.fst
@@ -1,0 +1,21 @@
+module ASN1.Low.NULL
+
+open ASN1.Base
+open ASN1.Spec.NULL
+open ASN1.Low.Base
+
+open FStar.Integers
+
+module HS = FStar.HyperStack
+module HST = FStar.HyperStack.ST
+module MB = LowStar.Monotonic.Buffer
+module B = LowStar.Buffer
+module Cast = FStar.Int.Cast
+
+let serialize32_asn1_null_backwards ()
+: Tot (serializer32_backwards serialize_asn1_null)
+= fun (_: unit)
+    (#rrel #rel: _)
+    (b: B.mbuffer byte_t rrel rel)
+    (pos: size_t)
+-> 0ul
