src/asn1/ASN1.Low.OCTET_STRING.fst
@@ -1,0 +1,69 @@
+module ASN1.Low.OCTET_STRING
+
+open ASN1.Base
+open ASN1.Spec.OCTET_STRING
+open ASN1.Low.Base
+open LowParse.Bytes
+
+open FStar.Integers
+
+module HS = FStar.HyperStack
+module HST = FStar.HyperStack.ST
+module MB = LowStar.Monotonic.Buffer
+module B = LowStar.Buffer
+module Cast = FStar.Int.Cast
+
+let serialize32_asn1_octet_string
+  (len: size_t)
+: Tot (serializer32 (serialize_asn1_octet_string (v len)))
+= fun (s: lbytes_t (v len))
+    (#rrel #rel: _)
+    (b: B.mbuffer byte_t rrel rel)
+    (pos: size_t)
+->  store_seqbytes
+    (* src *) s
+    (* from*) 0ul
+    (* to  *) len
+    (* dst *) b
+    (* pos *) pos;
+(* retuen *) len
+
+let serialize32_asn1_octet_string_backwards
+  (len: size_t)
+: Tot (serializer32_backwards (serialize_asn1_octet_string (v len)))
+= fun (s: lbytes_t (v len))
+    (#rrel #rel: _)
+    (b: B.mbuffer byte_t rrel rel)
+    (pos: size_t)
+->  (* Prf *) let h0 = HST.get () in
+
+    store_seqbytes
+    (* src *) s
+    (* from*) 0ul
+    (* to  *) len
+    (* dst *) b
+    (* pos *) (pos - len);
+
+    (* Prf *) let h1 = HST.get () in
+    (* Prf *) B.modifies_buffer_from_to_elim
+              (* buf *) b
+              (*frame*) 0ul (pos - len)
+              (* new *) (B.loc_buffer_from_to
+                         (* buf *) b
+                         (*range*) (pos - len) (pos))
+              (* mem *) h0 h1;
+    (* Prf *) B.modifies_buffer_from_to_elim
+              (* buf *) b
+              (*frame*) pos (u (B.length b))
+              (* new *) (B.loc_buffer_from_to
+                         (* buf *) b
+                         (*range*) (pos - len) (pos))
+              (* mem *) h0 h1;
+    (* Prf *) writable_modifies
+              (* buf *) b
+              (* new *) (v (pos - len)) (v (pos))
+              (* mem *) h0
+              (* loc *) B.loc_none
+              (* mem'*) h1;
+
+(* retuen *) len
