src/asn1/ASN1.Spec.Length.fst
@@ -1,0 +1,23 @@
+module ASN1.Spec.Length
+
+open LowParse.Spec.Base
+open LowParse.Spec.Combinators
+open LowParse.Spec.DER
+
+open ASN1.Base
+
+let asn1_int32 = bounded_int32 asn1_length_min asn1_length_max
+
+let parse_asn1_length_kind = parse_bounded_der_length32_kind asn1_length_min asn1_length_max
+
+let parse_asn1_length
+: parser parse_asn1_length_kind asn1_int32
+= parse_bounded_der_length32 asn1_length_min asn1_length_max
+
+let parse_asn1_length_unfold = parse_bounded_der_length32_unfold asn1_length_min asn1_length_max
+
+let serialize_asn1_length
+: serializer parse_asn1_length
+= serialize_bounded_der_length32 asn1_length_min asn1_length_max
+
+let serialize_asn1_length_unfold = serialize_bounded_der_length32_unfold asn1_length_min asn1_length_max
