src/asn1/ASN1.Spec.OCTET_STRING.fst
@@ -1,0 +1,11 @@
+module ASN1.Spec.OCTET_STRING
+
+open LowParse.Spec.Base
+open LowParse.Spec.Combinators
+open LowParse.Spec.SeqBytes.Base
+
+open ASN1.Base
+
+let parse_asn1_octet_string = parse_seq_flbytes
+
+let serialize_asn1_octet_string = serialize_seq_flbytes
